vale/code/arch/x64/interop/Simplify_Sha.fst
@@ -2,8 +2,9 @@ module Simplify_Sha
 
 friend SHA_helpers
 
-
 open Words_s
+
+#set-options "--z3rlimit 20"
 
 let reveal_get128 (s:Seq.lseq UInt8.t 16) (v0 v1 v2 v3:UInt32.t) : Lemma
   (requires 
