vale/code/arch/x64/interop/Vale.AsLowStar.MemoryHelpers.fst
@@ -31,10 +31,10 @@ let reveal_readable (#t:_) (x:buf_t t) (s:ME.mem) = ()
 let reveal_imm_readable (#t:_) (x:ibuf_t t) (s:ME.mem) = ()
 let readable_live (#t:_) (x:buf_t t) (s:ME.mem) = ()
 let readable_imm_live (#t:_) (x:ibuf_t t) (s:ME.mem) = ()
-let buffer_readable_reveal #n bt x args h0 stack = ()
-let get_heap_mk_mem_reveal #n args h0 stack = ()
-let buffer_as_seq_reveal #n t x args h0 stack = ()
-let immbuffer_as_seq_reveal #n t x args h0 stack = ()
+let buffer_readable_reveal #max_arity #n bt x args h0 stack = ()
+let get_heap_mk_mem_reveal #max_arity #n args h0 stack = ()
+let buffer_as_seq_reveal #max_arity #n t x args h0 stack = ()
+let immbuffer_as_seq_reveal #max_arity #n t x args h0 stack = ()
 let buffer_as_seq_reveal2 t x va_s = ()
 let immbuffer_as_seq_reveal2 t x va_s = ()
 let buffer_addr_reveal t x args h0 = ()
@@ -49,15 +49,17 @@ let modifies_equal_domains s h0 h1 = ()
 let loc_disjoint_sym (x y:ME.loc)  = ()
 
 let core_create_lemma_taint_hyp
+    #max_arity
+    #arg_reg
     #n
-    (args:IX64.arity_ok arg)
+    (args:IX64.arity_ok max_arity arg)
     (h0:HS.mem)
     (stack:IX64.stack_buffer n{mem_roots_p h0 (arg_of_sb stack::args)})
   : Lemma
-      (ensures (let va_s = LSig.create_initial_vale_state args h0 stack in
+      (ensures (let va_s = LSig.create_initial_vale_state #max_arity #arg_reg args h0 stack in
                 LSig.taint_hyp args va_s /\
                 ME.valid_taint_buf64 (as_vale_buffer stack) va_s.VS.mem va_s.VS.memTaint X64.Machine_s.Public))
-  = let va_s = LSig.create_initial_vale_state args h0 stack in
+  = let va_s = LSig.create_initial_vale_state #max_arity #arg_reg args h0 stack in
     let taint_map = va_s.VS.memTaint in
     let s_args = arg_of_sb stack::args in
     let mem = va_s.VS.mem in
